simplified yield type chcking and added treiber stack (not fully done)

Source/Concurrency/LinearSets.cs
@@ -154,6 +154,16 @@ namespace Microsoft.Boogie
         }
         public override Implementation VisitImplementation(Implementation node)
         {
+            node.PruneUnreachableBlocks();
+            node.ComputePredecessorsForBlocks();
+            GraphUtil.Graph<Block> graph = Program.GraphFromImpl(node);
+            graph.ComputeLoops();
+            if (!graph.Reducible)
+            {
+                Error(node, "A loop in the implementation is not reducible");
+                return node;
+            }
+
             HashSet<Variable> start = new HashSet<Variable>(globalVarToDomainName.Keys);
             for (int i = 0; i < node.InParams.Count; i++)
             {
@@ -223,6 +233,15 @@ namespace Microsoft.Boogie
                     }
                 }
             }
+
+            foreach (Block header in graph.Headers)
+            {
+                foreach (GlobalVariable g in globalVarToDomainName.Keys.Except(availableLinearVars[header]))
+                {
+                    Error(header, string.Format("Global variable {0} must be available at a loop head", g.Name));
+                }
+            }
+
             return impl;
         }
         public void AddAvailableVars(CallCmd callCmd, HashSet<Variable> start)
@@ -564,6 +583,12 @@ namespace Microsoft.Boogie
             foreach (Variable v in AvailableLinearVars(absy))
             {
                 var domainName = FindDomainName(v);
+                domainNameToScope[domainName].Add(v);
+            }
+            foreach (Variable v in program.GlobalVariables())
+            {
+                var domainName = FindDomainName(v);
+                if (domainName == null) continue;
                 domainNameToScope[domainName].Add(v);
             }
             foreach (string domainName in linearDomains.Keys)
