Source/Concurrency/YieldTypeChecker.cs
@@ -13,91 +13,109 @@ namespace Microsoft.Boogie
 {
     class YieldTypeChecker
     {
-        static List<Tuple<int, int, int>> yieldTypeCheckerAutomatonEdges;
+        static List<Tuple<int, int, int>> ASpec;
+        static List<Tuple<int, int, int>> BSpec;
+        static List<Tuple<int, int, int>> CSpec;
         static YieldTypeChecker()
         {
-            yieldTypeCheckerAutomatonEdges = new List<Tuple<int, int, int>>();
-            AddEdge(0, 'P', 0);
-            AddEdge(0, 'Y', 0);
-            AddEdge(0, 'Y', 1);
-            AddEdge(0, 'Y', 2);
-            AddEdge(1, 'P', 1);
-            AddEdge(1, 'R', 1);
-            AddEdge(1, 'B', 1);
-            AddEdge(1, 'Y', 1);
-            AddEdge(1, 'Y', 0);
-            AddEdge(1, 'A', 2);
-            AddEdge(1, 'P', 2);
-            AddEdge(1, 'R', 2);
-            AddEdge(1, 'B', 2);
-            AddEdge(1, 'Y', 2);
-            AddEdge(2, 'L', 2);
-            AddEdge(2, 'B', 2);
-            AddEdge(2, 'P', 2);
-            AddEdge(2, 'Y', 2);
-            AddEdge(2, 'Y', 1);
-            AddEdge(2, 'Y', 0);
-        }
-        private static void AddEdge(int source, int label, int dest)
-        {
-            yieldTypeCheckerAutomatonEdges.Add(new Tuple<int, int, int>(source, label, dest));
+            // initial: 0, final: 1
+            ASpec = new List<Tuple<int,int,int>>();
+            ASpec.Add(new Tuple<int, int, int>(0, 'Y', 1));
+            ASpec.Add(new Tuple<int, int, int>(1, 'Y', 1));
+            ASpec.Add(new Tuple<int, int, int>(1, 'B', 1));
+            ASpec.Add(new Tuple<int, int, int>(1, 'R', 1));
+            ASpec.Add(new Tuple<int, int, int>(1, 'L', 1));
+            ASpec.Add(new Tuple<int, int, int>(1, 'A', 1));
+            ASpec.Add(new Tuple<int, int, int>(0, 'P', 0));
+            ASpec.Add(new Tuple<int, int, int>(1, 'P', 1));
+
+            // initial: 1, final: 0
+            BSpec = new List<Tuple<int, int, int>>();
+            BSpec.Add(new Tuple<int, int, int>(1, 'Y', 0));
+            BSpec.Add(new Tuple<int, int, int>(1, 'Y', 1));
+            BSpec.Add(new Tuple<int, int, int>(1, 'B', 1));
+            BSpec.Add(new Tuple<int, int, int>(1, 'R', 1));
+            BSpec.Add(new Tuple<int, int, int>(1, 'L', 1));
+            BSpec.Add(new Tuple<int, int, int>(1, 'A', 1));
+            BSpec.Add(new Tuple<int, int, int>(0, 'P', 0));
+            BSpec.Add(new Tuple<int, int, int>(1, 'P', 1));
+
+            // initial: {0, 1}, final: {0, 1}
+            CSpec = new List<Tuple<int,int,int>>();
+            CSpec.Add(new Tuple<int, int, int>(0, 'B', 0));
+            CSpec.Add(new Tuple<int, int, int>(0, 'R', 0));
+            CSpec.Add(new Tuple<int, int, int>(0, 'Y', 0));
+            CSpec.Add(new Tuple<int, int, int>(0, 'B', 1));
+            CSpec.Add(new Tuple<int, int, int>(0, 'R', 1));
+            CSpec.Add(new Tuple<int, int, int>(0, 'L', 1));
+            CSpec.Add(new Tuple<int, int, int>(0, 'A', 1));
+            CSpec.Add(new Tuple<int, int, int>(1, 'B', 1));
+            CSpec.Add(new Tuple<int, int, int>(1, 'L', 1));
+            CSpec.Add(new Tuple<int, int, int>(1, 'Y', 0));
+            CSpec.Add(new Tuple<int, int, int>(0, 'P', 0));
+            CSpec.Add(new Tuple<int, int, int>(1, 'P', 1));
         }
 
         private void IsYieldTypeSafe()
         {
-            List<int[]> transitions = new List<int[]>();
-            foreach (Tuple<int, int> e in edgeLabels.Keys)
-            {
-                int label = edgeLabels[e];
-                int[] transition = new int[4];
-                transition[0] = e.Item1;
-                transition[1] = label;
-                transition[2] = label;
-                transition[3] = e.Item2;
-                transitions.Add(transition);
-            }
-
-            int dummyInitial = stateCounter;
-            foreach (Tuple<int, int> e in edgeLabels.Keys)
-            {
-                if (initialStates.Contains(e.Item1))
-                {
-                    int[] transition = new int[4];
-                    transition[0] = dummyInitial;
-                    transition[1] = edgeLabels[e];
-                    transition[2] = edgeLabels[e];
-                    transition[3] = e.Item2;
-                    transitions.Add(transition);
-                }
-            }
-
             List<Tuple<int, int, int>> implEdges = new List<Tuple<int, int, int>>();
-            foreach (int[] transition in transitions)
+            foreach (Tuple<int, int> e in edgeLabels.Keys)
             {
-                implEdges.Add(new Tuple<int, int, int>(transition[0], transition[1], transition[3]));
+                implEdges.Add(new Tuple<int, int, int>(e.Item1, edgeLabels[e], e.Item2));
             }
+            //Console.WriteLine(PrintGraph(impl, implEdges, initialState, finalStates));
+            ASpecCheck(implEdges);
+            BSpecCheck(implEdges);
+            CSpecCheck(implEdges);
+        }
+
+        private void ASpecCheck(List<Tuple<int, int, int>> implEdges)
+        {
             Dictionary<int, HashSet<int>> initialConstraints = new Dictionary<int, HashSet<int>>();
-            initialConstraints[dummyInitial] = new HashSet<int>(new int[] {0});
+            initialConstraints[initialState] = new HashSet<int>(new int[] { 0 });
+            foreach (var finalState in finalStates)
+            {
+                initialConstraints[finalState] = new HashSet<int>(new int[] { 1 });
+            }
+            SimulationRelation<int, int, int> x = new SimulationRelation<int, int, int>(implEdges, ASpec, initialConstraints);
+            Dictionary<int, HashSet<int>> simulationRelation = x.ComputeSimulationRelation();
+            if (simulationRelation[initialState].Count == 0)
+            {
+                moverTypeChecker.Error(impl, string.Format("Implementation {0} fails simulation check A at phase {1}. An action must be preceded by a yield.\n", impl.Name, currPhaseNum));
+            }
+        }
+
+        private void BSpecCheck(List<Tuple<int, int, int>> implEdges)
+        {
+            Dictionary<int, HashSet<int>> initialConstraints = new Dictionary<int, HashSet<int>>();
+            initialConstraints[initialState] = new HashSet<int>(new int[] { 1 });
             foreach (var finalState in finalStates)
             {
                 initialConstraints[finalState] = new HashSet<int>(new int[] { 0 });
             }
+            SimulationRelation<int, int, int> x = new SimulationRelation<int, int, int>(implEdges, BSpec, initialConstraints);
+            Dictionary<int, HashSet<int>> simulationRelation = x.ComputeSimulationRelation();
+            if (simulationRelation[initialState].Count == 0)
+            {
+                moverTypeChecker.Error(impl, string.Format("Implementation {0} fails simulation check B at phase {1}. An action must be succeeded by a yield.\n", impl.Name, currPhaseNum));
+            }
+        }
+
+        private void CSpecCheck(List<Tuple<int, int, int>> implEdges)
+        {
+            Dictionary<int, HashSet<int>> initialConstraints = new Dictionary<int, HashSet<int>>();
             foreach (Block block in loopHeaders)
             {
                 if (!IsTerminatingLoopHeader(block))
                 {
-                    initialConstraints[absyToNode[block]] = new HashSet<int>(new int[] { 0, 1 });
+                    initialConstraints[absyToNode[block]] = new HashSet<int>(new int[] { 0 });
                 }
             }
-            SimulationRelation<int, int, int> x = new SimulationRelation<int, int, int>(implEdges, yieldTypeCheckerAutomatonEdges, initialConstraints);
+            SimulationRelation<int, int, int> x = new SimulationRelation<int, int, int>(implEdges, CSpec, initialConstraints);
             Dictionary<int, HashSet<int>> simulationRelation = x.ComputeSimulationRelation();
-            foreach (Block block in loopHeaders)
+            if (simulationRelation[initialState].Count == 0)
             {
-                if (simulationRelation[absyToNode[block]].Count == 0)
-                {
-                    IToken tok = block.tok;
-                    moverTypeChecker.Error(impl, string.Format("Loop at {0}({1}, {2}) not simulated appropriately at phase {3}\n", tok.filename, tok.line, tok.col, currPhaseNum));
-                }
+                moverTypeChecker.Error(impl, string.Format("Implementation {0} fails simulation check C at phase {1}. Transactions must be separated by a yield.\n", impl.Name, currPhaseNum));
             }
         }
 
@@ -138,7 +156,7 @@ namespace Microsoft.Boogie
         int currPhaseNum;
         Dictionary<Absy, int> absyToNode;
         Dictionary<int, Absy> nodeToAbsy;
-        HashSet<int> initialStates;
+        int initialState;
         HashSet<int> finalStates;
         Dictionary<Tuple<int, int>, int> edgeLabels;
         IEnumerable<Block> loopHeaders;
@@ -151,8 +169,7 @@ namespace Microsoft.Boogie
             this.loopHeaders = loopHeaders;
             this.stateCounter = 0;
             this.absyToNode = new Dictionary<Absy, int>();
-            this.initialStates = new HashSet<int>();
-            initialStates.Add(0);
+            this.initialState = 0;
             this.finalStates = new HashSet<int>();
             this.edgeLabels = new Dictionary<Tuple<int, int>, int>(); 
             
@@ -312,13 +329,35 @@ namespace Microsoft.Boogie
             }
         }
 
-        private static string PrintGraph(Implementation yTypeChecked, Graph<int> graph, Dictionary<Tuple<int, int>, string> edgeLabels)
+        private static string PrintGraph(Implementation impl, List<Tuple<int, int, int>> edges, int initialState, HashSet<int> finalStates)
         {
             var s = new StringBuilder();
-            s.AppendLine("\nImplementation " + yTypeChecked.Proc.Name + " digraph G {");
-            foreach (var e in graph.Edges)
-                s.AppendLine("  \"" + e.Item1.ToString() + "\" -- " + edgeLabels[e] + " --> " + "  \"" + e.Item2.ToString() + "\";");
+            s.AppendLine("\nImplementation " + impl.Proc.Name + " digraph G {");
+            foreach (var e in edges)
+            {
+                string label = "P";
+                switch (e.Item2)
+                {
+                    case 'P': label = "P"; break;
+                    case 'Y': label = "Y"; break;
+                    case 'B': label = "B"; break;
+                    case 'R': label = "R"; break;
+                    case 'L': label = "L"; break;
+                    case 'A': label = "A"; break;
+                    default: Debug.Assert(false); break;
+                }
+                s.AppendLine("  \"" + e.Item1.ToString() + "\" -- " + label + " --> " + "  \"" + e.Item3.ToString() + "\";");
+            }
             s.AppendLine("}");
+            s.AppendLine("Initial state: " + initialState);
+            s.Append("Final states: ");
+            bool first = true;
+            foreach (int finalState in finalStates)
+            { 
+                s.Append((first ? "" : ", ") + finalState);
+                first = false;
+            }
+            s.AppendLine();
             return s.ToString();
         }
     }
