Test/og/Program1.bpl
@@ -15,11 +15,15 @@ ensures {:phase 1} x >= 8;
     yield;
     assert {:phase 1} x >= 7;
     call Incr(1); 
+    yield;
+    assert {:phase 1} x >= 8; 
 }
 
 procedure {:yields} {:phase 1} q() 
 { 
+    yield;
     call Incr(3); 
+    yield;
 }
 
 procedure {:yields} {:phase 0,1} Incr(val: int);
