Test/og/lock2.bpl
@@ -7,12 +7,10 @@ procedure {:yields} {:phase 2} main()
     yield;
     while (*)
     {
-        yield;
-
         async call Customer();
-
         yield;
     }
+    yield;
 }
 
 procedure {:yields} {:phase 2} Customer()
@@ -20,16 +18,12 @@ procedure {:yields} {:phase 2} Customer()
     yield;
     while (*) 
     {
-    	yield;
-
         call Enter();
-
     	yield;
-
     	call Leave();
-
         yield;
     }
+    yield;
 }
 
 procedure {:yields} {:phase 1,2} Enter() 
@@ -38,21 +32,21 @@ ensures {:atomic} |{ A: assume b == 0; b := 1; return true; }|;
     var _old, curr: int;
     yield;
     while (true) { 
-    	yield;
         call _old := CAS(0, 1);
 	yield;
         if (_old == 0) {
-	    return;
+	    break;
 	}
 	while (true) {
-	    yield;
 	    call curr := Read();
 	    yield;
 	    if (curr == 0) {
 	        break;
 	    }
 	}
+	yield;
     }
+    yield;
 }
 
 procedure {:yields} {:phase 0,2} Read() returns (val: int);
